<?xml version="1.0" encoding="utf-8"?>
<rdf:RDF xmlns:rdf="http://www.w3.org/1999/02/22-rdf-syntax-ns#"
         xmlns:crm="http://www.cidoc-crm.org/cidoc-crm/"
         xmlns:dcterms="http://purl.org/dc/terms/"
         xmlns:foaf="http://xmlns.com/foaf/0.1/"
         xmlns:geo="http://www.w3.org/2003/01/geo/wgs84_pos#"
         xmlns:kid="https://kerameikos.org/id/"
         xmlns:kon="https://kerameikos.org/ontology#"
         xmlns:lexinfo="http://www.lexinfo.net/ontology/2.0/lexinfo#"
         xmlns:ontolex="http://www.w3.org/ns/lemon/ontolex#"
         xmlns:org="http://www.w3.org/ns/org#"
         xmlns:osgeo="http://data.ordnancesurvey.co.uk/ontology/geometry/"
         xmlns:owl="http://www.w3.org/2002/07/owl#"
         xmlns:prov="http://www.w3.org/ns/prov#"
         xmlns:rdfs="http://www.w3.org/2000/01/rdf-schema#"
         xmlns:skos="http://www.w3.org/2004/02/skos/core#"
         xmlns:un="http://www.owl-ontologies.com/Ontology1181490123.owl#"
         xmlns:xsd="http://www.w3.org/2001/XMLSchema#">
    <kon:Shape rdf:about="https://kerameikos.org/id/psykter-amphora">
        <rdf:type rdf:resource="http://www.w3.org/2004/02/skos/core#Concept"/>
        <skos:inScheme rdf:resource="https://kerameikos.org/id/"/>
        <skos:prefLabel xml:lang="en">Psykter Amphora</skos:prefLabel>
        <skos:broader rdf:resource="https://kerameikos.org/id/amphora"/>
        <skos:broader rdf:resource="https://kerameikos.org/id/psykter"/>
        <skos:definition xml:lang="en">The psykter-amphora is a double-walled container whose walls are attached at the neck and at the base, the outer vessel having a spout at the shoulder through which ice or ice water was poured into the space between the two walls. It usually has a drain spout just above the foot, directly below the pour spout. The shape was probably only produced in the 6th c. BCE.</skos:definition>
        <dcterms:source rdf:resource="https://zenon.dainst.org/Record/000188572"/>
        <skos:exactMatch rdf:resource="https://www.britishmuseum.org/collection/term/x8609"/>
        <skos:exactMatch rdf:resource="http://vocab.getty.edu/aat/300264973"/>
        <skos:changeNote rdf:resource="https://kerameikos.org/id/psykter-amphora#provenance"/>
        <skos:prefLabel xml:lang="de">Psykter Amphore</skos:prefLabel>
        <skos:definition xml:lang="de">Die Psykter Amphore ist ein doppelwandiger Behälter dessen Wände am Hals und Fuß verbunden sind. Der äußere Gefäßkörper hat einen Ausguß, der zur Befüllung des Zwischenraums mit Eis oder Eiswasser gedient hat. Es hat üblicherweise einen Ausguß oberhalb vom Fuß. Die Gefäßform wurde wahrscheinlich nur im 6. Jh.n.Chr. produziert.</skos:definition>
        <skos:prefLabel xml:lang="el">ψυκτήρας-αμφορέας</skos:prefLabel>
        <skos:definition xml:lang="el">Ο ψυκτήρας-αμφορέας είναι ένα αγγείο με διπλά τοιχώματα, τα οποία προσαρτώνται στον λαιμό και στη βάση. Στην εξωτερική επιφάνεια του αγγείου υπάρχει μια προχοή, μέσω της οποίας γέμιζαν το διάστημα ανάμεσα στα δύο τοιχώματα με πάγο ή παγωμένο νερό. Διαθέτει συνήθως και μια προχοή απορροής, πάνω από το πόδι. Το σχήμα παραγόταν πιθανώς μόνο κατά τον 6ο αι. π. X.</skos:definition>
        <skos:definition xml:lang="he">אמפורת הפסיקטר היא מיכל בעל דופן כפולה, שדפנותיו מחוברות באזור הצוואר ובתחתית. לחלק החיצוני של הכלי יש פיה/זרבובית באזור הכתף, שדרכה הוכנס קרח או מי קרח אל המרווח שבין שתי הדפנות. לרוב יש לו גם פיית ניקוז ממש מעל לתחתית, ישירות מתחת לפיית המזיגה. נראה שצורה זו יוצרה רק במאה ה-6 לפנה״ס.</skos:definition>
    </kon:Shape>
   
   
    <dcterms:ProvenanceStatement rdf:about="https://kerameikos.org/id/psykter-amphora#provenance">
					   <foaf:topic rdf:resource="https://kerameikos.org/id/psykter-amphora"/>
				    <prov:wasGeneratedBy>
            <prov:Activity>
                <rdf:type rdf:resource="http://www.w3.org/ns/prov#Create"/>
					           <prov:atTime rdf:datatype="http://www.w3.org/2001/XMLSchema#dateTime">2019-03-21T18:13:46.127-04:00</prov:atTime>
					           <prov:wasAssociatedWith rdf:resource="https://kerameikos.org/editor/egruber"/>
					           <prov:used rdf:resource="https://docs.google.com/spreadsheets/d/1p6TKXjCQe-C3DNhGFdh7g6Th7RbMg9lMueDYsdfMj-c/pubhtml"/>
					           <dcterms:type>spreadsheet</dcterms:type>
				        </prov:Activity>
        </prov:wasGeneratedBy>
        <prov:activity>
            <prov:Activity>
                <rdf:type rdf:resource="http://www.w3.org/ns/prov#Modify"/>
					           <prov:atTime rdf:datatype="http://www.w3.org/2001/XMLSchema#dateTime">2019-09-23T13:31:54.701-04:00</prov:atTime>
					           <prov:wasAssociatedWith rdf:resource="https://kerameikos.org/editor/egruber"/>
					           <prov:used rdf:resource="https://docs.google.com/spreadsheets/d/1p6TKXjCQe-C3DNhGFdh7g6Th7RbMg9lMueDYsdfMj-c/pubhtml"/>
					           <dcterms:type>spreadsheet</dcterms:type>
				        </prov:Activity>
        </prov:activity>
        <prov:activity>
            <prov:Activity>
                <rdf:type rdf:resource="http://www.w3.org/ns/prov#Modify"/>
					           <prov:atTime rdf:datatype="http://www.w3.org/2001/XMLSchema#dateTime">2021-03-12T10:47:04.304-05:00</prov:atTime>
					           <prov:wasAssociatedWith rdf:resource="https://kerameikos.org/editor/egruber"/>
					           <prov:used rdf:resource="https://docs.google.com/spreadsheets/d/1p6TKXjCQe-C3DNhGFdh7g6Th7RbMg9lMueDYsdfMj-c/pubhtml"/>
					           <dcterms:type>spreadsheet</dcterms:type>
				        </prov:Activity>
        </prov:activity>
        <prov:activity>
            <prov:Activity>
                <rdf:type rdf:resource="http://www.w3.org/ns/prov#Modify"/>
					           <prov:atTime rdf:datatype="http://www.w3.org/2001/XMLSchema#dateTime">2025-08-19T19:18:07.445Z</prov:atTime>
					           <prov:wasAssociatedWith rdf:resource="https://kerameikos.org/editor/egruber"/>
					           <prov:used rdf:resource="https://docs.google.com/spreadsheets/d/1p6TKXjCQe-C3DNhGFdh7g6Th7RbMg9lMueDYsdfMj-c/pubhtml"/>
					           <dcterms:type>spreadsheet</dcterms:type>
				        </prov:Activity>
        </prov:activity>
    </dcterms:ProvenanceStatement>
</rdf:RDF>