<?xml version="1.0" encoding="utf-8"?>
<rdf:RDF xmlns:rdf="http://www.w3.org/1999/02/22-rdf-syntax-ns#"
         xmlns:crm="http://www.cidoc-crm.org/cidoc-crm/"
         xmlns:dcterms="http://purl.org/dc/terms/"
         xmlns:foaf="http://xmlns.com/foaf/0.1/"
         xmlns:geo="http://www.w3.org/2003/01/geo/wgs84_pos#"
         xmlns:kid="http://kerameikos.org/id/"
         xmlns:kon="http://kerameikos.org/ontology#"
         xmlns:lexinfo="http://www.lexinfo.net/ontology/2.0/lexinfo#"
         xmlns:ontolex="http://www.w3.org/ns/lemon/ontolex#"
         xmlns:org="http://www.w3.org/ns/org#"
         xmlns:osgeo="http://data.ordnancesurvey.co.uk/ontology/geometry/"
         xmlns:owl="http://www.w3.org/2002/07/owl#"
         xmlns:prov="http://www.w3.org/ns/prov#"
         xmlns:rdfs="http://www.w3.org/2000/01/rdf-schema#"
         xmlns:skos="http://www.w3.org/2004/02/skos/core#"
         xmlns:un="http://www.owl-ontologies.com/Ontology1181490123.owl#"
         xmlns:xsd="http://www.w3.org/2001/XMLSchema#">
    <kon:Shape rdf:about="http://kerameikos.org/id/psykter-calyx_krater">
        <rdf:type rdf:resource="http://www.w3.org/2004/02/skos/core#Concept"/>
        <skos:inScheme rdf:resource="http://kerameikos.org/id/"/>
        <skos:prefLabel xml:lang="en">Psykter Calyx Krater</skos:prefLabel>
        <skos:broader rdf:resource="http://kerameikos.org/id/calyx_krater"/>
        <skos:broader rdf:resource="http://kerameikos.org/id/psykter"/>
        <skos:definition xml:lang="en">Rarer than but similar to the psykter-amphora, the psykter-calyx-krater is a double-walled vessel meant to cool wine or water. The outer vessel has a spout near the shoulder through which ice or ice water was poured into the space between the two walls. It usually has a drain spout just above the foot, directly below the pour spout.</skos:definition>
        <dcterms:source rdf:resource="https://zenon.dainst.org/Record/000926820"/>
        <skos:changeNote rdf:resource="http://kerameikos.org/id/psykter-calyx_krater#provenance"/>
        <skos:prefLabel xml:lang="de">Psykter Kelchkrater</skos:prefLabel>
        <skos:definition xml:lang="de">Der Psykter Kelchkrater ist seltener aber ähnlich der Psykter Amhore. Der doppelwandige Behälter wurde zum kühlen von Wein oder Wasser verwendet. Der äußere Gefäßkörper hat einen Ausguß nahe der Schulter, der zur Befüllung des Zwischenraums zwischen den Wänden mit Eis oder Eiswasser gedient hat. Es hat üblicherweise einen Ausguß oberhalb vom Fuß.</skos:definition>
        <skos:prefLabel xml:lang="el">ψυκτήρας-καλυκωτός κρατήρας</skos:prefLabel>
        <skos:definition xml:lang="el">Σπανιότερος, ωστόσο παρόμοιος με τον ψυκτήρα-αμφορεά, ο ψυκτήρας-καλυκωτός κρατήρας είναι ένα αγγείο με διπλά τοιχώματα για να διατηρείται δροσερός ο κεκραμένος οίνος. Στο εξωτερικό τοίχωμα του αγγείου υπάρχει μια προχοή κοντά στον ώμo, ενώ συνήθως διαθέτει μια προχοή απορροής ακριβώς πάνω από το πόδι.</skos:definition>
        <skos:definition xml:lang="he">נדיר יותר אך דומה לאמפורת הפסיקטר, הפסיקטר-קאליקס-קרטר הוא כלי בעל דופן כפולה שנועד לקרר יין או מים. לכלי החיצוני יש פיה סמוך לכתף, שדרכה הוכנס קרח או מי קרח אל החלל שבין שתי הדפנות. לרוב יש לו גם פיית ניקוז ממש מעל לבסיס, ישירות מתחת לפיית המזיגה.</skos:definition>
    </kon:Shape>
   
   
    <dcterms:ProvenanceStatement rdf:about="http://kerameikos.org/id/psykter-calyx_krater#provenance">
					   <foaf:topic rdf:resource="http://kerameikos.org/id/psykter-calyx_krater"/>
				    <prov:wasGeneratedBy>
            <prov:Activity>
                <rdf:type rdf:resource="http://www.w3.org/ns/prov#Create"/>
					           <prov:atTime rdf:datatype="http://www.w3.org/2001/XMLSchema#dateTime">2019-03-21T18:13:46.127-04:00</prov:atTime>
					           <prov:wasAssociatedWith rdf:resource="http://kerameikos.org/editor/egruber"/>
					           <prov:used rdf:resource="https://docs.google.com/spreadsheets/d/1p6TKXjCQe-C3DNhGFdh7g6Th7RbMg9lMueDYsdfMj-c/pubhtml"/>
					           <dcterms:type>spreadsheet</dcterms:type>
				        </prov:Activity>
        </prov:wasGeneratedBy>
        <prov:activity>
            <prov:Activity>
                <rdf:type rdf:resource="http://www.w3.org/ns/prov#Modify"/>
					           <prov:atTime rdf:datatype="http://www.w3.org/2001/XMLSchema#dateTime">2019-09-23T13:31:54.701-04:00</prov:atTime>
					           <prov:wasAssociatedWith rdf:resource="http://kerameikos.org/editor/egruber"/>
					           <prov:used rdf:resource="https://docs.google.com/spreadsheets/d/1p6TKXjCQe-C3DNhGFdh7g6Th7RbMg9lMueDYsdfMj-c/pubhtml"/>
					           <dcterms:type>spreadsheet</dcterms:type>
				        </prov:Activity>
        </prov:activity>
        <prov:activity>
            <prov:Activity>
                <rdf:type rdf:resource="http://www.w3.org/ns/prov#Modify"/>
					           <prov:atTime rdf:datatype="http://www.w3.org/2001/XMLSchema#dateTime">2021-03-12T10:47:04.304-05:00</prov:atTime>
					           <prov:wasAssociatedWith rdf:resource="http://kerameikos.org/editor/egruber"/>
					           <prov:used rdf:resource="https://docs.google.com/spreadsheets/d/1p6TKXjCQe-C3DNhGFdh7g6Th7RbMg9lMueDYsdfMj-c/pubhtml"/>
					           <dcterms:type>spreadsheet</dcterms:type>
				        </prov:Activity>
        </prov:activity>
        <prov:activity>
            <prov:Activity>
                <rdf:type rdf:resource="http://www.w3.org/ns/prov#Modify"/>
					           <prov:atTime rdf:datatype="http://www.w3.org/2001/XMLSchema#dateTime">2025-08-19T19:18:07.445Z</prov:atTime>
					           <prov:wasAssociatedWith rdf:resource="http://kerameikos.org/editor/egruber"/>
					           <prov:used rdf:resource="https://docs.google.com/spreadsheets/d/1p6TKXjCQe-C3DNhGFdh7g6Th7RbMg9lMueDYsdfMj-c/pubhtml"/>
					           <dcterms:type>spreadsheet</dcterms:type>
				        </prov:Activity>
        </prov:activity>
    </dcterms:ProvenanceStatement>
</rdf:RDF>