<?xml version="1.0" encoding="UTF-8"?>
<rdf:RDF xmlns:rdf="http://www.w3.org/1999/02/22-rdf-syntax-ns#" xmlns:crm="http://www.cidoc-crm.org/cidoc-crm/" xmlns:owl="http://www.w3.org/2002/07/owl#"
	xmlns:dcterms="http://purl.org/dc/terms/" xmlns:xsd="http://www.w3.org/2001/XMLSchema#" xmlns:rdfs="http://www.w3.org/2000/01/rdf-schema#" xmlns:kon="http://kerameikos.org/ontology#">
	<owl:Ontology rdf:about="http://kerameikos.org/ontology#">
		<rdfs:label xml:lang="en">Kerameikos.org Ontology</rdfs:label>
		<dcterms:created rdf:datatype="http://www.w3.org/2001/XMLSchema#date">2014-07-21</dcterms:created>
		<dcterms:modified rdf:datatype="http://www.w3.org/2001/XMLSchema#date">2021-11-17</dcterms:modified>
		<rdfs:comment xml:lang="en">Ontology for defining classes and properties that apply to ceramics as extensions to CIDOC-CRM.</rdfs:comment>
		<dcterms:creator rdf:resource="https://orcid.org/0000-0002-4691-9747"/>
		<rdfs:seeAlso rdf:resource="http://kerameikos.org/ontology"/>
		<owl:versionInfo>1.0</owl:versionInfo>
	</owl:Ontology>
	<!-- classes -->
	<owl:Class rdf:about="http://kerameikos.org/ontology#Shape">
		<rdfs:label xml:lang="en">Shape</rdfs:label>
		<rdfs:comment xml:lang="en">The form of an object can be expressed as specific terminology, e.g. 'olpe', or in generic terms, 'pitcher'. Scholars of
			ceramics typically refer to this form as the 'shape' of a vessel, whereas museum catalogers classify the form as an 'object type'.</rdfs:comment>
		<rdfs:subClassOf rdf:resource="http://www.cidoc-crm.org/cidoc-crm/E55_Type"/>
		<rdf:type rdf:resource="http://www.w3.org/2000/01/rdf-schema#Class"/>
		<rdfs:isDefinedBy rdf:resource="http://kerameikos.org/ontology"/>
	</owl:Class>
	<owl:Class rdf:about="http://kerameikos.org/ontology#Style">
		<rdfs:label xml:lang="en">Style</rdfs:label>
		<rdfs:comment xml:lang="en">Illustrative motif on a vessel, whether decorative or figural. A style often has a cultural and/or period component.</rdfs:comment>
		<rdfs:subClassOf rdf:resource="http://www.cidoc-crm.org/cidoc-crm/E55_Type"/>
		<rdf:type rdf:resource="http://www.w3.org/2000/01/rdf-schema#Class"/>
		<rdfs:isDefinedBy rdf:resource="http://kerameikos.org/ontology"/>
	</owl:Class>
	<owl:Class rdf:about="http://kerameikos.org/ontology#Technique">
		<rdfs:label xml:lang="en">Technique</rdfs:label>
		<rdfs:comment xml:lang="en">The technical method by which a vessel is formed, decorated, and/or fired. Complex techniques, such as black-figure, may comprise more than one technique.</rdfs:comment>
		<rdfs:subClassOf rdf:resource="http://www.cidoc-crm.org/cidoc-crm/E55_Type"/>
		<rdf:type rdf:resource="http://www.w3.org/2000/01/rdf-schema#Class"/>
		<rdfs:isDefinedBy rdf:resource="http://kerameikos.org/ontology"/>
	</owl:Class>
	<!--<owl:Class rdf:about="http://kerameikos.org/ontology#Ware">
		<rdfs:label xml:lang="en">Ware</rdfs:label>
		<rdfs:comment xml:lang="en">Stub for the description of Ware</rdfs:comment>
		<rdfs:subClassOf rdf:resource="http://www.cidoc-crm.org/cidoc-crm/E55_Type"/>
		<rdf:type rdf:resource="http://www.w3.org/2000/01/rdf-schema#Class"/>
		<rdfs:isDefinedBy rdf:resource="http://kerameikos.org/ontology"/>
	</owl:Class>-->
	<!-- properties -->
	<owl:ObjectProperty rdf:about="http://kerameikos.org/ontology#hasShape">
		<rdfs:label xml:lang="en">Has Shape</rdfs:label>
		<rdfs:comment xml:lang="en">A physical object (vase or other ceramic vessel) has a shape, defined by a resource of kon:Shape class.</rdfs:comment>
		<rdfs:subPropertyOf rdf:resource="http://www.cidoc-crm.org/cidoc-crm/P2_has_type"/>
		<rdfs:domain rdf:resource="http://www.cidoc-crm.org/cidoc-crm/E22_Human-Made_Object"/>
		<rdfs:range rdf:resource="http://kerameikos.org/ontology#Shape"/>
		<rdf:type rdf:resource="http://www.w3.org/1999/02/22-rdf-syntax-ns#Property"/>
	</owl:ObjectProperty>
</rdf:RDF>
