@prefix rdf: <http://www.w3.org/1999/02/22-rdf-syntax-ns#> .
@prefix crm: <http://www.cidoc-crm.org/cidoc-crm/> .
@prefix owl: <http://www.w3.org/2002/07/owl#> .
@prefix dcterms: <http://purl.org/dc/terms/> .
@prefix xsd: <http://www.w3.org/2001/XMLSchema#> .
@prefix rdfs: <http://www.w3.org/2000/01/rdf-schema#> .
@prefix kon: <https://kerameikos.org/ontology#> .

<https://kerameikos.org/ontology#>
    dcterms:created "2014-07-21"^^xsd:date ;
    dcterms:creator <https://orcid.org/0000-0002-4691-9747> ;
    dcterms:modified "2021-11-17"^^xsd:date ;
    a owl:Ontology ;
    rdfs:comment "Ontology for defining classes and properties that apply to ceramics as extensions to CIDOC-CRM."@en ;
    rdfs:label "Kerameikos.org Ontology"@en ;
    rdfs:seeAlso <https://kerameikos.org/ontology> ;
    owl:versionInfo "1.0" .

kon:Shape
    a rdfs:Class, owl:Class ;
    rdfs:comment """The form of an object can be expressed as specific terminology, e.g. 'olpe', or in generic terms, 'pitcher'. Scholars of
			ceramics typically refer to this form as the 'shape' of a vessel, whereas museum catalogers classify the form as an 'object type'."""@en ;
    rdfs:isDefinedBy <https://kerameikos.org/ontology> ;
    rdfs:label "Shape"@en ;
    rdfs:subClassOf crm:E55_Type .

kon:Style
    a rdfs:Class, owl:Class ;
    rdfs:comment "Illustrative motif on a vessel, whether decorative or figural. A style often has a cultural and/or period component."@en ;
    rdfs:isDefinedBy <https://kerameikos.org/ontology> ;
    rdfs:label "Style"@en ;
    rdfs:subClassOf crm:E55_Type .

kon:Technique
    a rdfs:Class, owl:Class ;
    rdfs:comment "The technical method by which a vessel is formed, decorated, and/or fired. Complex techniques, such as black-figure, may comprise more than one technique."@en ;
    rdfs:isDefinedBy <https://kerameikos.org/ontology> ;
    rdfs:label "Technique"@en ;
    rdfs:subClassOf crm:E55_Type .

kon:hasShape
    a rdf:Property, owl:ObjectProperty ;
    rdfs:comment "A physical object (vase or other ceramic vessel) has a shape, defined by a resource of kon:Shape class."@en ;
    rdfs:domain crm:E22_Human-Made_Object ;
    rdfs:label "Has Shape"@en ;
    rdfs:range kon:Shape ;
    rdfs:subPropertyOf crm:P2_has_type .

