@prefix rdf: <http://www.w3.org/1999/02/22-rdf-syntax-ns#> .
@prefix skos: <http://www.w3.org/2004/02/skos/core#> .
@prefix foaf: <http://xmlns.com/foaf/0.1/> .
@prefix kon: <https://kerameikos.org/ontology#> .
@prefix owl: <http://www.w3.org/2002/07/owl#> .
@prefix dcterms: <http://purl.org/dc/terms/> .
@prefix xsd: <http://www.w3.org/2001/XMLSchema#> .
@prefix rdfs: <http://www.w3.org/2000/01/rdf-schema#> .

<https://kerameikos.org/ontology#>
    dcterms:contributor [
        foaf:mbox "ewg4xuva@gmail.com" ;
        foaf:name "Ethan Gruber"
    ] ;
    dcterms:created "2014-07-21"^^xsd:date ;
    a owl:Ontology ;
    rdfs:comment """Vocabulary for defining classes and properties that apply to ceramics, filling in gaps left between existing ontologies, such as
            CIDOC-CRM"""@en ;
    rdfs:label "Kerameikos.org Ontology"@en ;
    rdfs:seeAlso <https://kerameikos.org/ontology> ;
    owl:versionInfo "0.1" .

kon:ProductionPlace
    a owl:Class ;
    rdfs:comment "Stub for the description of Production Place, as a concept. To be differentiated from ecrm:E53_Place and geo:SpatialThing, which are physical locations."@en ;
    rdfs:isDefinedBy <https://kerameikos.org/ontology> ;
    rdfs:label "Production Place"@en ;
    rdfs:subClassOf skos:Concept .

kon:Shape
    a owl:Class ;
    rdfs:comment "Stub for the description of Shape"@en ;
    rdfs:isDefinedBy <https://kerameikos.org/ontology> ;
    rdfs:label "Shape"@en ;
    rdfs:subClassOf skos:Concept .

kon:Style
    a owl:Class ;
    rdfs:comment "Stub for the description of Style"@en ;
    rdfs:isDefinedBy <https://kerameikos.org/ontology> ;
    rdfs:label "Style"@en ;
    rdfs:subClassOf skos:Concept .

kon:Technique
    a owl:Class ;
    rdfs:comment "Stub for the description of Technique"@en ;
    rdfs:isDefinedBy <https://kerameikos.org/ontology> ;
    rdfs:label "Technique"@en ;
    rdfs:subClassOf skos:Concept .

kon:Ware
    a owl:Class ;
    rdfs:comment "Stub for the description of Ware"@en ;
    rdfs:isDefinedBy <https://kerameikos.org/ontology> ;
    rdfs:label "Ware"@en ;
    rdfs:subClassOf skos:Concept .

kon:hasShape
    a rdf:Property, owl:ObjectProperty ;
    rdfs:comment "A physical object (vase or other ceramic vessel) has a shape, defined by a resource of kon:Shape class."@en ;
    rdfs:domain kon:Shape ;
    rdfs:label "Has Shape"@en ;
    rdfs:range <http://erlangen-crm.org/140617/E18_Physical_Thing> .

